examples/mw/MWApp1New.v
@@ -16,7 +16,7 @@ Set Implicit Arguments.
 
 Section PROOF.
 
-  Context `{@GRA.inG AppRA Σ}.
+  Context `{@GRA.inG AppRA.t Σ}.
 
   Notation pget := (p0 <- trigger PGet;; p0 <- p0↓ǃ;; Ret p0) (only parsing).
   Notation pput p0 := (trigger (PPut p0↑)) (only parsing).
@@ -61,14 +61,14 @@ Section PROOF.
      rf := choose (rf - rm - ro)
    ***)
 
-  Definition ASSUME rf0 (P: AppRA -> Prop): itree Es _ :=
+  Definition ASSUME rf0 (P: AppRA.t -> Prop): itree Es _ :=
     ri <- trigger (Take _);;
     assume(P ri);;;
     rm <- pget;; rf1 <- trigger (Take _);; assume(rf1 = rm ⋅ ri ⋅ rf0 ∧ URA.wf rf1);;;
     Ret rf1
   .
 
-  Definition GUARANTEE rf0 (Q: AppRA -> Prop): itree Es _ :=
+  Definition GUARANTEE rf0 (Q: AppRA.t -> Prop): itree Es _ :=
     '(rm, ro, rf1) <- trigger (Choose _);;
     guarantee(Q ro);;;
     guarantee(rm ⋅ ro ⋅ rf1 = rf0);;; pput rm;;;
@@ -78,13 +78,13 @@ Section PROOF.
   Definition initF: list val -> itree Es val :=
     fun varg => _ <- (pargs [] varg)?;;
       let rf := ε in
-      rf <- (ASSUME rf (eq AppInit));;
+      rf <- (ASSUME rf (eq Init));;
 
       rf <- (GUARANTEE rf top1);;
       `_: val <- ccallU "put" [Vint 0; Vint 42];;
       rf <- (ASSUME rf top1);;
 
-      rf <- (GUARANTEE rf (eq AppRun));;
+      rf <- (GUARANTEE rf (eq Run));;
 
       Ret Vundef
   .
@@ -107,20 +107,20 @@ Section PROOF.
   Definition runF: list val -> itree Es val :=
     fun varg => _ <- (pargs [] varg)?;;
       let rf := ε in
-      rf <- (ASSUME rf (eq AppRun));;
+      rf <- (ASSUME rf (eq Run));;
 
       rf <- (GUARANTEE rf top1);;
       `v: val <- ccallU "get" [Vint 0];; trigger (Syscall "print" [v]↑ top1);;;
       rf <- (ASSUME rf top1);;
 
-      rf <- GUARANTEE rf (eq AppRun);;
+      rf <- GUARANTEE rf (eq Run);;
       Ret Vundef
   .
 
   Definition AppSem: ModSem.t := {|
     ModSem.fnsems := [("init", cfunU initF); ("run", cfunU runF)];
     ModSem.mn := "App";
-    ModSem.initial_st := (AppInitX)↑;
+    ModSem.initial_st := (InitX)↑;
   |}
   .
 
